Added refinement to enforce that certain closed expressions are values in the rules (so you don't need to carry the proof around) and proved that reflexive step for destruct EPair implies that it is a value

rupicola/stlc/STLC.fst
@@ -266,10 +266,9 @@ type step : closed_exp -> closed_exp -> Type =
     hst:step e1 e1' ->
     step (EPair e1 e2) (EPair e1' e2)
   | PairRight :
-    e1:closed_exp ->
+    e1:closed_exp{is_value e1} ->
     #e2:closed_exp ->
     #e2':closed_exp ->
-    is_value e1 ->
     hst:step e2 e2' ->
     step (EPair e1 e2) (EPair e1 e2')
   | FstPair :
@@ -278,8 +277,8 @@ type step : closed_exp -> closed_exp -> Type =
     hst:step e' e'' ->
     step (EFst e') (EFst e'')
   | FstPairReturn :
-    #e1:value ->
-    #e2:value ->
+    #e1:closed_exp{is_value e1} ->
+    #e2:closed_exp{is_value e2} ->
     step (EFst (EPair e1 e2)) e1
   | SndPair :
     #e':closed_exp ->
@@ -287,8 +286,8 @@ type step : closed_exp -> closed_exp -> Type =
     hst:step e' e'' ->
     step (ESnd e') (ESnd e'')
   | SndPairReturn :
-    #e1:closed_exp -> (* why doesn´t this work with value like I did for FstPairReturn? *)
-    #e2:closed_exp ->
+    #e1:closed_exp{is_value e1} ->
+    #e2:closed_exp{is_value e2} ->
     step (ESnd (EPair e1 e2)) e2
 
 let can_step (e:closed_exp) : Type0 =
@@ -318,7 +317,7 @@ let rec lem_value_is_irred (e:closed_exp) : Lemma
         FStar.Squash.bind_squash #(step e e') () (fun st ->
         match st with
         | PairLeft e2 hst -> ()
-        | PairRight e1 is_val_e1 hst -> ()
+        | PairRight e1 hst -> ()
         | _ -> ())
       end
     end
@@ -610,6 +609,31 @@ let rec destruct_steps_eif
       EIf e1 e2 e3 -->* EIf e1' e2 e3 -->* e'
   **)
 
+let srefl_epair_implies_value (e1 e2:closed_exp) : Lemma
+  (requires safe e1 /\ safe e2 /\ irred (EPair e1 e2))
+  (ensures is_value (EPair e1 e2))
+  =
+  introduce irred e1 /\ irred e2 ==> is_value (EPair e1 e2) with _.
+  begin () end;
+  introduce ~(irred e1) ==> is_value (EPair e1 e2) with _.
+  begin
+    assert (exists e1'. step e1 e1');
+    eliminate exists e1'. step e1 e1' returns exists e'. step (EPair e1 e2) e' with st.
+    begin
+      bind_squash st (fun st -> return_squash (PairLeft e2 st))
+    end;
+    false_elim ()
+  end;
+  introduce irred e1 /\ ~(irred e2) ==> is_value (EPair e1 e2) with _.
+  begin
+    assert (exists e2'. step e2 e2');
+    eliminate exists e2'. step e2 e2' returns exists e'. step (EPair e1 e2) e' with st.
+    begin
+      bind_squash st (fun st -> return_squash (PairRight e1 st))
+    end;
+    false_elim ()
+  end
+
 let rec destruct_steps_epair
   (e1:closed_exp)
   (e2:closed_exp)
@@ -628,7 +652,7 @@ let rec destruct_steps_epair
     (decreases st)
   = match st with
     | SRefl (EPair e1 e2) -> begin
-      assume (is_value e1 /\ is_value e2);
+      srefl_epair_implies_value e1 e2;
       (e1, e2)
       end
     | STrans #f1 #f2 #f3 step_epair step_epair_steps -> begin
@@ -646,7 +670,7 @@ let rec destruct_steps_epair
         lem_steps_transitive (EPair e1 e2) (EPair e1' e2) (EPair e1'' e2'');
         (e1'', e2'')
         end
-      | PairRight e1 #e2 #e2' is_val_e1 step_e2 -> begin
+      | PairRight e1 #e2 #e2' step_e2 -> begin
         let (EPair e1 e2') = f2 in
         lem_step_implies_steps e2 e2';
         lem_step_implies_steps (EPair e1 e2) (EPair e1 e2');
@@ -808,7 +832,6 @@ let rec destruct_steps_epair_snd
       end
     | SndPairReturn #e1 #e2 -> begin
       lem_step_implies_steps (ESnd (EPair e1 e2)) e2;
-      assume (is_value e12);
       e12
       end
     | _ -> false_elim ()
